EvmAsm/Rv64/WordOps.lean
@@ -64,7 +64,7 @@ theorem generic_lwu_spec (rd rs1 : Reg) (v_addr v_old : Word)
     (holdsFor_regIs _ _ s).mp (holdsFor_sepConj_elim_left
       (holdsFor_sepConj_elim_left hPR))
   have hmem : s.getMem dwordAddr = word_val :=
-    (holdsFor_memIs _ _ s).mp (holdsFor_sepConj_elim_right (holdsFor_sepConj_elim_right
+    holdsFor_memIs_getMem (holdsFor_sepConj_elim_right (holdsFor_sepConj_elim_right
       (holdsFor_sepConj_elim_left hPR)))
   have hstep' : step s = some (execInstrBr s (.LWU rd rs1 offset)) :=
     step_lwu s rd rs1 offset hfetch (hrs1 ▸ hvalid)
@@ -109,7 +109,7 @@ theorem generic_lw_spec (rd rs1 : Reg) (v_addr v_old : Word)
     (holdsFor_regIs _ _ s).mp (holdsFor_sepConj_elim_left
       (holdsFor_sepConj_elim_left hPR))
   have hmem : s.getMem dwordAddr = word_val :=
-    (holdsFor_memIs _ _ s).mp (holdsFor_sepConj_elim_right (holdsFor_sepConj_elim_right
+    holdsFor_memIs_getMem (holdsFor_sepConj_elim_right (holdsFor_sepConj_elim_right
       (holdsFor_sepConj_elim_left hPR)))
   have hstep' : step s = some (execInstrBr s (.LW rd rs1 offset)) :=
     step_lw s rd rs1 offset hfetch (hrs1 ▸ hvalid)
@@ -155,7 +155,7 @@ theorem generic_sw_spec (rs1 rs2 : Reg) (v_addr v_data : Word)
     (holdsFor_regIs _ _ s).mp (holdsFor_sepConj_elim_left (holdsFor_sepConj_elim_right
       (holdsFor_sepConj_elim_left hPR)))
   have hmem : s.getMem dwordAddr = word_old :=
-    (holdsFor_memIs _ _ s).mp (holdsFor_sepConj_elim_right (holdsFor_sepConj_elim_right
+    holdsFor_memIs_getMem (holdsFor_sepConj_elim_right (holdsFor_sepConj_elim_right
       (holdsFor_sepConj_elim_left hPR)))
   have hstep' : step s = some (execInstrBr s (.SW rs1 rs2 offset)) :=
     step_sw s rs1 rs2 offset hfetch (hrs1 ▸ hvalid)
